src/SDK/MessageHeader.dfy
@@ -1,5 +1,6 @@
 include "AlgorithmSuite.dfy"
 include "../StandardLibrary/StandardLibrary.dfy"
+include "EncryptionContext.dfy"
 include "Materials.dfy"
 include "../Util/UTF8.dfy"
 include "../Util/Sets.dfy"
@@ -9,17 +10,10 @@ module {:extern "MessageHeader"} MessageHeader {
   import Sets
   import opened StandardLibrary
   import opened UInt = StandardLibrary.UInt
+  import EncryptionContext
   import Materials
   import UTF8
 
-
-  // To make verification and working with iterating through the encryption context
-  // simpler, here we define a specific type to represent a sequence of key-value tuples.
-  type EncryptionContextSeq = seq<(UTF8.ValidUTF8Bytes, UTF8.ValidUTF8Bytes)>
-
-  // There isn't an efficient way to build a map from a sequence in dafny, so this
-  // extern is used specifically to convert a sequence of key value pairs to a map
-  method {:extern "KVPairSequenceToMap"} KVPairSequenceToMap(kvPairs: EncryptionContextSeq) returns (res: Materials.EncryptionContext)
 
   /*
    * Definition of the message header, i.e., the header body and the header authentication
@@ -85,14 +79,14 @@ module {:extern "MessageHeader"} MessageHeader {
                           typ: Type,
                           algorithmSuiteID: AlgorithmSuite.ID,
                           messageID: MessageID,
-                          aad: Materials.EncryptionContext,
+                          aad: EncryptionContext.Map,
                           encryptedDataKeys: EncryptedDataKeys,
                           contentType: ContentType,
                           ivLength: uint8,
                           frameLength: uint32)
   {
     predicate Valid() {
-      && ValidAAD(aad)
+      && EncryptionContext.Valid(aad)
       && encryptedDataKeys.Valid()
       && algorithmSuiteID.IVLength() == ivLength as nat
       && ValidFrameLength(frameLength, contentType)
@@ -105,206 +99,10 @@ module {:extern "MessageHeader"} MessageHeader {
 
   datatype HeaderAuthentication = HeaderAuthentication(iv: seq<uint8>, authenticationTag: seq<uint8>)
 
-  /*
-   * Validity predicates -- predicates that say when the data structures above are in a good state.
-   */
-
-  predicate ValidKVPair(kvPair: (UTF8.ValidUTF8Bytes, UTF8.ValidUTF8Bytes)) {
-    && |kvPair.0| < UINT16_LIMIT
-    && |kvPair.1| < UINT16_LIMIT
-    && UTF8.ValidUTF8Seq(kvPair.0)
-    && UTF8.ValidUTF8Seq(kvPair.1)
-  }
-
-  // Length of KVPairEntries is defined in terms of a seq of tuples, which is easier to reason about
-  function KVPairEntriesLength(kvPairs: EncryptionContextSeq, lo: nat, hi: nat): nat
-    requires lo <= hi <= |kvPairs|
-  {
-    if lo == hi then 0 else
-      KVPairEntriesLength(kvPairs, lo, hi - 1) +
-      2 + |kvPairs[hi - 1].0| +
-      2 + |kvPairs[hi - 1].1|
-  }
-
-  lemma KVPairEntriesLengthSplit(kvPairs: EncryptionContextSeq, lo: nat, mid: nat, hi: nat)
-    requires lo <= mid <= hi <= |kvPairs|
-    ensures KVPairEntriesLength(kvPairs, lo, hi)
-         == KVPairEntriesLength(kvPairs, lo, mid) + KVPairEntriesLength(kvPairs, mid, hi)
-  {
-  }
-
-  lemma KVPairEntriesLengthPrefix(kvPairs: EncryptionContextSeq, more: EncryptionContextSeq)
-    ensures KVPairEntriesLength(kvPairs + more, 0, |kvPairs|) == KVPairEntriesLength(kvPairs, 0, |kvPairs|)
-  {
-    var n := |kvPairs|;
-    if n == 0 {
-    } else {
-      var last := kvPairs[n - 1];
-      calc {
-        KVPairEntriesLength(kvPairs + more, 0, n);
-      ==  // def. KVPairEntriesLength
-        KVPairEntriesLength(kvPairs + more, 0, n - 1) + 4 + |last.0| + |last.1|;
-      ==  { assert kvPairs + more == kvPairs[..n - 1] + ([last] + more); }
-        KVPairEntriesLength(kvPairs[..n - 1] + ([last] + more), 0, n - 1) + 4 + |last.0| + |last.1|;
-      ==  { KVPairEntriesLengthPrefix(kvPairs[..n - 1], [last] + more); }
-        KVPairEntriesLength(kvPairs[..n - 1], 0, n - 1) + 4 + |last.0| + |last.1|;
-      ==  { KVPairEntriesLengthPrefix(kvPairs[..n - 1], [last] + more); }
-        KVPairEntriesLength(kvPairs[..n - 1] + [last], 0, n - 1) + 4 + |last.0| + |last.1|;
-      ==  { assert kvPairs[..n - 1] + [last] == kvPairs; }
-        KVPairEntriesLength(kvPairs, 0, n - 1) + 4 + |last.0| + |last.1|;
-      ==  // def. KVPairEntriesLength
-        KVPairEntriesLength(kvPairs, 0, n);
-      }
-    }
-  }
-
-  lemma KVPairEntriesLengthExtend(kvPairs: EncryptionContextSeq, key: UTF8.ValidUTF8Bytes, value: UTF8.ValidUTF8Bytes)
-    ensures KVPairEntriesLength(kvPairs + [(key, value)], 0, |kvPairs| + 1)
-         == KVPairEntriesLength(kvPairs, 0, |kvPairs|) + 4 + |key| + |value|
-  {
-    KVPairEntriesLengthPrefix(kvPairs, [(key, value)]);
-  }
-
-  lemma KVPairEntriesLengthInsert(kvPairs: EncryptionContextSeq, insertionPoint: nat, key: UTF8.ValidUTF8Bytes, value: UTF8.ValidUTF8Bytes)
-    requires insertionPoint <= |kvPairs|
-    ensures var kvPairs' := kvPairs[..insertionPoint] + [(key, value)] + kvPairs[insertionPoint..];
-      KVPairEntriesLength(kvPairs', 0, |kvPairs'|) == KVPairEntriesLength(kvPairs, 0, |kvPairs|) + 4 + |key| + |value|
-    decreases |kvPairs|
-  {
-    var kvPairs' := kvPairs[..insertionPoint] + [(key, value)] + kvPairs[insertionPoint..];
-    if |kvPairs| == insertionPoint {
-      assert kvPairs' == kvPairs + [(key, value)];
-      KVPairEntriesLengthExtend(kvPairs, key, value);
-    } else {
-      var m := |kvPairs| - 1;
-      var (d0, d1) := kvPairs[m];
-      var a, b, c, d := kvPairs[..insertionPoint], [(key, value)], kvPairs[insertionPoint..m], [(d0, d1)];
-      assert kvPairs == a + c + d;
-      assert kvPairs' == a + b + c + d;
-      var ac := a + c;
-      var abc := a + b + c;
-      calc {
-        KVPairEntriesLength(kvPairs', 0, |kvPairs'|);
-        KVPairEntriesLength(abc + [(d0, d1)], 0, |abc| + 1);
-      ==  { KVPairEntriesLengthExtend(abc, d0, d1); }
-        KVPairEntriesLength(abc, 0, |abc|) + 4 + |d0| + |d1|;
-      ==  { KVPairEntriesLengthInsert(ac, insertionPoint, key, value); }
-        KVPairEntriesLength(ac, 0, |ac|) + 4 + |key| + |value| + 4 + |d0| + |d1|;
-      ==  { KVPairEntriesLengthExtend(ac, d0, d1); }
-        KVPairEntriesLength(kvPairs, 0, |kvPairs|) + 4 + |key| + |value|;
-      }
-    }
-  }
-
-  function KVPairsLength(encryptionContext: Materials.EncryptionContext): nat 
-  {
-    if |encryptionContext| == 0 then 0 else
-      // Defining and reasoning about order at this level is simplified by using a sequence of
-      // key value pairs instead of a map.
-      var keys: seq<UTF8.ValidUTF8Bytes> := SetToOrderedSequence(encryptionContext.Keys, UInt.UInt8Less);
-      var kvPairs := seq(|keys|, i requires 0 <= i < |keys| => (keys[i], encryptionContext[keys[i]]));
-      2 + KVPairEntriesLength(kvPairs, 0, |kvPairs|)
-  }
-
-  method ComputeKVPairsLength(encryptionContext: Materials.EncryptionContext) returns (res: nat)
-    ensures res as nat == KVPairsLength(encryptionContext)
-  {
-    reveal ValidAAD();
-    if |encryptionContext| == 0 {
-      return 0;
-    }
-
-    // Iterating through a map isn't feasbile in dafny for large maps, so instead
-    // convert the map to a sequence of key pairs and iterate through the sequence
-    var keys: seq<UTF8.ValidUTF8Bytes> := Sets.ComputeSetToOrderedSequence(encryptionContext.Keys, UInt.UInt8Less);
-    var kvPairs := seq(|keys|, i requires 0 <= i < |keys| => (keys[i], encryptionContext[keys[i]]));
-
-    var len := 2;
-    var i := 0;
-    while i < |kvPairs|
-      invariant i <= |kvPairs|
-      invariant 2 + KVPairEntriesLength(kvPairs, 0, i as int) == len as int
-    {
-      var kvPair := kvPairs[i];
-      len := len + 4 + |kvPair.0| + |kvPair.1|;
-      KVPairEntriesLengthSplit(kvPairs, 0, i + 1, |kvPairs| as int);
-      i := i + 1;
-    }
-
-    assert len == 2 + KVPairEntriesLength(kvPairs, 0, |kvPairs|);
-    assert len == KVPairsLength(encryptionContext);
-
-    return len;
-  }
-
-  predicate {:opaque} ValidAAD(encryptionContext: Materials.EncryptionContext) {
-    && KVPairsLength(encryptionContext) < UINT16_LIMIT
-    && ValidKVPairs(encryptionContext)
-  }
-
-  method ComputeValidAAD(encryptionContext: Materials.EncryptionContext) returns (res: bool)
-    ensures res == ValidAAD(encryptionContext)
-  {
-    reveal ValidAAD();
-
-    if |encryptionContext| == 0 {
-      return true;
-    } else if |encryptionContext| >= UINT16_LIMIT {
-      return false;
-    }
-    
-    // Iterating through a map isn't feasbile in dafny for large maps, so instead
-    // convert the map to a sequence of key pairs and iterate through the sequence
-    var keys: seq<UTF8.ValidUTF8Bytes> := Sets.ComputeSetToOrderedSequence<uint8>(encryptionContext.Keys, UInt.UInt8Less);
-    var kvPairs := seq(|keys|, i requires 0 <= i < |keys| => (keys[i], encryptionContext[keys[i]]));
-    assert forall i :: 0 <= i < |keys| ==> kvPairs[i] == (keys[i], encryptionContext[keys[i]]);
-
-    var kvPairsLen := 2;
-    var i := 0;
-    while i < |kvPairs|
-      invariant i <= |kvPairs|
-      invariant forall k :: 0 <= k < i ==> ValidKVPair(kvPairs[k])
-      invariant 2 + KVPairEntriesLength(kvPairs, 0, i as int) == kvPairsLen as int < UINT16_LIMIT
-    {
-      var kvPair := kvPairs[i];
-      kvPairsLen := kvPairsLen + 4 + |kvPair.0| + |kvPair.1|;
-      KVPairEntriesLengthSplit(kvPairs, 0, i as int + 1, |kvPairs| as int);
-
-      // Check that AAD is still valid with this pair
-      if !(|kvPair.0| < UINT16_LIMIT && |kvPair.1| < UINT16_LIMIT) {
-        assert kvPair.0 in encryptionContext.Keys;
-        return false; // Invalid key value pair
-      } else if kvPairsLen >= UINT16_LIMIT {
-        return false; // Over size limit
-      }
-      assert forall k :: 0 <= k < i ==> ValidKVPair(kvPairs[k]);
-      assert kvPairsLen < UINT16_LIMIT;
-      i := i + 1;
-    }
-
-    return true;
-  }
-
-  predicate ValidKVPairs(encryptionContext: Materials.EncryptionContext) {
-    && |encryptionContext| < UINT16_LIMIT
-    && (forall key :: key in encryptionContext.Keys ==> ValidKVPair((key, encryptionContext[key])))
-  }
-
   predicate ValidFrameLength(frameLength: uint32, contentType: ContentType) {
     match contentType
     case NonFramed => frameLength == 0
     case Framed => frameLength != 0
-  }
-
-  predicate SortedKVPairsUpTo(a: EncryptionContextSeq, n: nat)
-    requires n <= |a|
-  {
-    forall j :: 0 < j < n ==> LexicographicLessOrEqual(a[j-1].0, a[j].0, UInt.UInt8Less)
-  }
-
-  predicate SortedKVPairs(kvPairs: EncryptionContextSeq)
-  {
-    SortedKVPairsUpTo(kvPairs, |kvPairs|)
   }
 
   /*
@@ -318,52 +116,12 @@ module {:extern "MessageHeader"} MessageHeader {
     [hb.typ as uint8] +
     UInt16ToSeq(hb.algorithmSuiteID as uint16) +
     hb.messageID +
-    AADToSeq(hb.aad) +
+    EncryptionContext.MapToLinear(hb.aad) +
     EDKsToSeq(hb.encryptedDataKeys) +
     [ContentTypeToUInt8(hb.contentType)] +
     Reserved +
     [hb.ivLength] +
     UInt32ToSeq(hb.frameLength)
-  }
-
-  function AADToSeq(kvPairs: Materials.EncryptionContext): seq<uint8>
-    requires ValidAAD(kvPairs)
-  {
-    reveal ValidAAD();
-    UInt16ToSeq(KVPairsLength(kvPairs) as uint16) +
-    KVPairsToSeq(kvPairs)
-  }
-
-  function KVPairsToSeq(kvPairs: Materials.EncryptionContext): seq<uint8>
-    requires ValidKVPairs(kvPairs)
-  {
-    var n := |kvPairs|;
-    if n == 0 then [] else
-      // Defining and reasoning about order at this level is simplified by using a sequence of
-      // key value pairs instead of a map.
-      // Pairs are ordered lexicographically by their UTF8 encoding, which is equivalent to code
-      // point ordering.
-      var keys: seq<UTF8.ValidUTF8Bytes> := SetToOrderedSequence<uint8>(kvPairs.Keys, UInt.UInt8Less);
-      var kvPairsSeq := seq(|keys|, i requires 0 <= i < |keys| => (keys[i], kvPairs[keys[i]]));
-      UInt16ToSeq(n as uint16) +
-      KVPairEntriesToSeq(kvPairsSeq, 0, |kvPairsSeq|)
-  }
-
-  // Serialization of KVPairEntries is defined in terms of a seq of tuples, which is easier to reason about
-  function KVPairEntriesToSeq(kvPairs: EncryptionContextSeq, lo: nat, hi: nat): seq<uint8>
-    requires forall i :: 0 <= i < |kvPairs| ==> ValidKVPair(kvPairs[i])
-    requires |kvPairs| < UINT16_LIMIT
-    requires SortedKVPairs(kvPairs)
-    requires lo <= hi <= |kvPairs|
-  {
-    if lo == hi then [] else KVPairEntriesToSeq(kvPairs, lo, hi - 1) + KVPairToSeq(kvPairs[hi - 1])
-  }
-
-  function KVPairToSeq(kvPair: (UTF8.ValidUTF8Bytes, UTF8.ValidUTF8Bytes)): seq<uint8>
-    requires ValidKVPair(kvPair)
-  {
-    UInt16ToSeq(|kvPair.0| as uint16) + kvPair.0 +
-    UInt16ToSeq(|kvPair.1| as uint16) + kvPair.1
   }
 
   function EDKsToSeq(encryptedDataKeys: EncryptedDataKeys): seq<uint8>
@@ -387,65 +145,5 @@ module {:extern "MessageHeader"} MessageHeader {
     UInt16ToSeq(|edk.providerID| as uint16)   + edk.providerID +
     UInt16ToSeq(|edk.providerInfo| as uint16) + edk.providerInfo +
     UInt16ToSeq(|edk.ciphertext| as uint16)   + edk.ciphertext
-  }
-
-  /* Function KVPairsLength is defined without referring to SerializeAAD (because then
-   * these two would be mutually recursive with ValidAAD). The following lemma proves
-   * that the two definitions correspond.
-   */
-
-  lemma ADDLengthCorrect(encryptionContext: Materials.EncryptionContext)
-    requires ValidAAD(encryptionContext)
-    ensures |AADToSeq(encryptionContext)| == 2 + KVPairsLength(encryptionContext)
-  {
-    reveal ValidAAD();
-    var keys: seq<UTF8.ValidUTF8Bytes> := SetToOrderedSequence(encryptionContext.Keys, UInt.UInt8Less);
-    var kvPairs := seq(|keys|, i requires 0 <= i < |keys| => (keys[i], encryptionContext[keys[i]]));
-    KVPairEntriesLengthCorrect(kvPairs, 0, |kvPairs|);
-    /**** Here's a more detailed proof:
-    var n := |kvPairs|;
-    if n != 0 {
-      var s := KVPairEntriesToSeq(kvPairs, 0, n);
-      calc {
-        |AADToSeq(kvPairs)|;
-      ==  // def. AADToSeq
-        |UInt16ToSeq(KVPairsLength(kvPairs) as uint16) + UInt16ToSeq(n as uint16) + s|;
-      ==  // UInt16ToSeq yields length-2 sequence
-        2 + 2 + |s|;
-      ==  { KVPairEntriesLengthCorrect(kvPairs, 0, n); }
-        2 + 2 + KVPairEntriesLength(kvPairs, 0, n);
-      }
-    }
-    ****/
-  }
-
-  lemma KVPairEntriesLengthCorrect(encryptionContext: EncryptionContextSeq, lo: nat, hi: nat)
-    requires forall i :: 0 <= i < |encryptionContext| ==> ValidKVPair(encryptionContext[i])
-    requires lo <= hi <= |encryptionContext|
-    requires |encryptionContext| < UINT16_LIMIT
-    requires SortedKVPairs(encryptionContext)
-    ensures |KVPairEntriesToSeq(encryptionContext, lo, hi)| == KVPairEntriesLength(encryptionContext, lo, hi)
-  {
-    /**** Here's a more detailed proof:
-    if lo < hi {
-      var kvPair := kvPairs[hi - 1];
-      calc {
-        |KVPairEntriesToSeq(kvPairs, lo, hi)|;
-      ==  // def. KVPairEntriesToSeq
-        |KVPairEntriesToSeq(kvPairs, lo, hi - 1) + KVPairToSeq(kvPair)|;
-      ==
-        |KVPairEntriesToSeq(kvPairs, lo, hi - 1)| + |KVPairToSeq(kvPair)|;
-      ==  { KVPairEntriesLengthCorrect(kvPairs, lo, hi - 1); }
-        KVPairEntriesLength(kvPairs, lo, hi - 1) + |KVPairToSeq(kvPair)|;
-      ==  // def. KVPairToSeq
-        KVPairEntriesLength(kvPairs, lo, hi - 1) +
-        |UInt16ToSeq(|kvPair.0| as uint16) + kvPair.0 + UInt16ToSeq(|kvPair.1| as uint16) + kvPair.1|;
-      ==
-        KVPairEntriesLength(kvPairs, lo, hi - 1) + 2 + |kvPair.0| + 2 + |kvPair.1|;
-      ==  // def. KVPairEntriesLength
-        KVPairEntriesLength(kvPairs, lo, hi);
-      }
-    }
-    ****/
   }
 }
